refactoring, documentation, and fixing the upper bound of the mod interval

xtext/org.archware.sosadl/src/org/archware/sosadl/validation/typing/proof/ProofTerm.java
@@ -16,7 +16,35 @@ import org.archware.sosadl.validation.typing.proof.fields.OptionalField;
 import org.eclipse.xtext.xbase.lib.ListExtensions;
 import org.eclipse.xtext.xbase.lib.StringExtensions;
 
+/**
+ * A Coq term reified as a Java object.
+ * 
+ * The default implementation uses Java reflexivity in order to generate the proper formatting.
+ * The {@link ProofTerm#getConstructorName()} method is used to generate the name of the Coq constructor.
+ * The {@link ProofTerm#getDeclaredFields()} method retrieves the fields of the object, i.e., the parameters of the Coq constructor.
+ * The {@link ProofTerm#describeField(Field)} method can be overridden in order to customized how each field is handled.
+ * 
+ * A typical usage scenario is:
+ * 
+ * {@code
+ * out = "(" + p.getConstructorName() + " "
+ *     + Stream.of(p.getDeclaredFiles())
+ *       .map(this::processField)
+ *       .collect(Collectors.joining(" "))
+ *     + ")";
+ * }
+ * 
+ * @author Jeremy Buisson
+ */
 public interface ProofTerm {
+	/**
+	 * Returns the name of the Coq constructor for this object.
+	 * 
+	 * Whenever the class is annotated with {@link CoqConstructor}, the returned name is the one in the {@link CoqConstructor#value()} field of the annotation.
+	 * Otherwise, the returned name is the name of the class, of which the first letter is turned to lower case.
+	 * 
+	 * @return name of the Coq constructor.
+	 */
 	default String getConstructorName() {
 		Class<?> c = this.getClass();
 		CoqConstructor cc = c.getAnnotation(CoqConstructor.class);
@@ -27,6 +55,16 @@ public interface ProofTerm {
 		}
 	}
 
+	/**
+	 * Returns an array containing the fields for this object.
+	 * 
+	 * Each field, which encodes one parameter in the corresponding Coq term, implements any of {@link Eluded}, {@link ListField}, {@link MandatoryField} or {@link OptionalField}, depending on the characteristics of the field.
+	 * The actual choice of what type is returned is delegated to the {@link #describeField(Field)} method, such that it can be customized by any implementing class.
+	 * 
+	 * The returned array is built from the one returned by {@link Class#getDeclaredFields()}.
+	 * 
+	 * @return array of the fields to be used as parameters in the Coq term.
+	 */
 	default FieldDescriptor[] getDeclaredFields() {
 		Class<?> c = this.getClass();
 		FieldDescriptor[] f = Stream.of(c.getDeclaredFields()).map(this::describeField)
@@ -34,6 +72,24 @@ public interface ProofTerm {
 		return f;
 	}
 
+	/**
+	 * Returns the value and description of a field to be used as a parameter in a Coq term.
+	 * 
+	 * Depending on the annotation and type of the field:
+	 * <ul>
+	 * <li>If the field is annotated with {@link Eluded}, then an {@link EludedField} is returned.</li>
+	 * <li>If the field has type {@link java.util.List} (or any subtype), then a  {@link ListField} is returned.</li>
+	 * <li>If the field is annotated with {@link Mandatory}, then a {@link MandatoryField} is returned.</li>
+	 * <li>Otherwise, a {@link OptionalField} is returned.</li>
+	 * </ul>
+	 * 
+	 * In the {@link ListField}, {@link MandatoryField} and {@link OptionalField} cases, if the field is is annotated with {@link CoqLiteral}, then the field is assumed to hold an instance of {@link CharSequence}.
+	 * This {@link CharSequence} is returned as it is, without any additional operation, by the {@link ListField#get(Function)}, {@link MandatoryField#get(Function)} and {@link OptionalField#get(Function)} methods, respectively.
+	 * 
+	 * @param f the field to process
+	 * 
+	 * @return the field value and description as expected in order to format the Coq code.
+	 */
 	default FieldDescriptor describeField(Field f) {
 		if (f.isAnnotationPresent(Eluded.class)) {
 			return new EludedField() {
@@ -46,7 +102,7 @@ public interface ProofTerm {
 			try {
 				Method getter = f.getDeclaringClass().getMethod("get" + StringExtensions.toFirstUpper(f.getName()));
 				Object content = getter.invoke(this);
-				if (List.class.isAssignableFrom(f.getType())) {
+				if ((content != null && content instanceof List) || List.class.isAssignableFrom(f.getType())) {
 					if (f.isAnnotationPresent(CoqLiteral.class)) {
 						return new ListField() {
 							@Override
@@ -75,7 +131,7 @@ public interface ProofTerm {
 						};
 					}
 				} else {
-					if (f.isAnnotationPresent(CoqLiteral.class) && CharSequence.class.isAssignableFrom(f.getType())) {
+					if (f.isAnnotationPresent(CoqLiteral.class)) {
 						Optional<CharSequence> c = Optional.ofNullable((CharSequence) content);
 						if (f.isAnnotationPresent(Mandatory.class)) {
 							return new MandatoryField() {
