xtext/org.archware.sosadl/src/org/archware/sosadl/validation/typing/proof/ProofTermPlaceHolder.java
@@ -1,0 +1,33 @@
+package org.archware.sosadl.validation.typing.proof;
+
+import java.lang.reflect.Field;
+import java.util.Optional;
+
+import org.archware.sosadl.validation.typing.proof.fields.FieldDescriptor;
+
+public class ProofTermPlaceHolder implements ProofTerm {
+	private Optional<ProofTerm> proxy;
+	
+	public ProofTermPlaceHolder() {
+		this.proxy = Optional.empty();
+	}
+	
+	public void fillWith(ProofTerm p) {
+		this.proxy = Optional.of(p);
+	}
+
+	@Override
+	public String getConstructorName() {
+		return this.proxy.get().getConstructorName();
+	}
+
+	@Override
+	public FieldDescriptor[] getDeclaredFields() {
+		return this.proxy.get().getDeclaredFields();
+	}
+
+	@Override
+	public FieldDescriptor describeField(Field f) {
+		return this.proxy.get().describeField(f);
+	}
+}
