xtext/org.archware.sosadl/src/org/archware/sosadl/validation/typing/proof/fields/ListField.java
@@ -4,6 +4,22 @@ import java.util.List;
 import java.util.Optional;
 import java.util.function.Function;
 
+import org.archware.sosadl.validation.typing.proof.CoqLiteral;
+
+/**
+ * A list field, containing a sequence of objects.
+ * 
+ * @author Jeremy Buisson
+ */
 public interface ListField extends FieldDescriptor {
-	List<Optional<CharSequence>> get(Function<Object, CharSequence> process);
+	/**
+	 * Retrieves and format the contained objects using the given function.
+	 * 
+	 * Note that the exact semantics depends on the implementing class.
+	 * For instance, an implementation for {@link CoqLiteral}-annotated fields would return the contained objects, without applying the formatter function.
+	 * 
+	 * @param formatter the function applied to each of the contained objects.
+	 * @return the list of formatted objects.
+	 */
+	List<Optional<CharSequence>> get(Function<Object, CharSequence> formatter);
 }
